going to try switching to sublist

src/library_dev_extras/util.lean
@@ -312,7 +312,7 @@ apply ne.symm,
 apply nodup_cons_neq H_in_xs H_nd,
 end
 
-lemma subset_nil {X : Type} {xs : list X} : xs ⊆ [] → xs = nil :=
+lemma subset_nil {X : Type*} {xs : list X} : xs ⊆ [] → xs = nil :=
 begin
 intros H_ss,
 dunfold has_subset.subset list.subset at H_ss,
@@ -325,9 +325,77 @@ exfalso,
 exact (not_mem_nil x) H_x
 end
 
-lemma nodup_append_subset₁ {X : Type} {ys zs : list X} : Π (xs : list X), nodup (ys ++ zs) → xs ⊆ ys → nodup (xs ++ zs)
-| [] := begin simp, intros H_nd H_ss, exact nodup_of_nodup_append_right H_nd, end
-| (x::xs) := sorry
+lemma subset_cons_nil {X : Type*} {xs : list X} {x : X} : ¬ (x :: xs ⊆ []) :=
+begin
+intro H_contra,
+note H := list.subset_nil H_contra,
+injection H
+end
+
+inductive is_subset_of {α : Type*} : list α → list α → Prop
+| base : ∀ xs, is_subset_of [] xs
+| addr : ∀ xs y ys, is_subset_of xs ys → is_subset_of xs (y :: ys)
+| addl : ∀ xs x ys, is_subset_of xs ys → x ∈ ys → is_subset_of (x :: xs) ys
+
+lemma is_subset_of_subset {α : Type*} : Π {xs ys : list α}, xs ⊆ ys → is_subset_of xs ys
+| []      _       H_ss := by apply is_subset_of.base
+| (x::xs) []      H_ss := by { rw (subset_nil H_ss), apply is_subset_of.base }
+| (x::xs) (y::ys) H_ss :=
+begin
+apply is_subset_of.addl,
+apply is_subset_of_subset,
+apply subset_of_cons_subset H_ss,
+dunfold has_subset.subset list.subset at H_ss,
+exact H_ss mem_of_cons_same
+end
+
+lemma cons_subset_of_mem_subset {α : Type*} : Π (xs ys : list α) (x : α), x ∈ ys → xs ⊆ ys → (x :: xs) ⊆ ys :=
+assume xs ys x H_in H_ss,
+begin
+intros y Hy_in,
+dunfold has_mem.mem list.mem at Hy_in,
+cases Hy_in with H_eq H_mem,
+subst H_eq, exact H_in,
+exact H_ss H_mem
+end
+
+set_option trace.eqn_compiler.wf_rec true
+lemma subset_of_is_subset_of {α : Type*} : Π {xs ys : list α}, is_subset_of xs ys → xs ⊆ ys
+| []      _       H_isso := nil_subset _
+| (x::xs) []      H_isso :=
+begin
+cases H_isso with _ _ _ _ _ _ _ _ _ H_contra H_isso₁,
+exfalso, apply not_mem_nil _ H_contra
+end
+
+| (x::xs) (y::ys) H_isso :=
+begin
+cases H_isso with _ _ H₁ H₂ H_isso₁ H₄ H₅ H₆ H_isso₁ H_in H_isso₂,
+apply subset_cons_of_subset _ (subset_of_is_subset_of H_isso₁),
+apply cons_subset_of_mem_subset,
+exact H_in,
+apply subset_of_is_subset_of H_isso₁
+end using_well_founded
+
+lemma not_mem_of_nodup_subset {α : Type*} {xs ys : list α} {x : α} : x :: xs ⊆ ys → nodup ys → x ∉ xs :=
+begin
+intros H_ss H_nd H_in,
+
+end
+
+lemma nodup_append_subset₁ {X : Type*} {ys zs : list X} : Π (xs : list X), nodup (ys ++ zs) → xs ⊆ ys → nodup (xs ++ zs) :=
+begin
+intros xs H_nd H_ss,
+note H_isso := is_subset_of_subset H_ss,
+induction H_isso with xs xs y ys H_ss₁ IH₁ xs x ys H_ss₂ H_in₂ IH₂,
+{ simp, exact nodup_of_nodup_append_right H_nd },
+{ apply IH₁, apply nodup_of_nodup_cons H_nd, exact subset_of_is_subset_of H_ss₁ },
+assert H_nd_xs_zs : nodup (xs ++ zs),
+{ exact IH₂ H_nd (subset_of_cons_subset H_ss) },
+simp,
+assert H_x_nin_xs : x ∉ xs,
+
+end
 
 lemma nodup_append_swap {X : Type} {xs₁ xs₂ : list X} {x : X} : nodup (xs₁ ++ (x :: xs₂)) → nodup ((x::xs₁) ++ xs₂) :=
 by apply list.nodup_head
